select

SPES.thy
@@ -2,7 +2,10 @@ theory SPES
   imports "HOL-Library.Multiset"
 begin
 
-datatype query = Table string
+datatype op = Plus | Minus
+datatype sql_expr = Column nat | SConst nat | Null | Bin sql_expr op sql_expr
+
+datatype query = Table string | Select query "sql_expr list"
 
 datatype svalue = SNull | SNat nat
 type_synonym row = "svalue list"
@@ -16,7 +19,21 @@ definition wellformed_table :: "table \<Rightarrow> nat \<Rightarrow> bool" wher
 definition wellformed_db :: "db \<Rightarrow> bool" where
 "wellformed_db db \<equiv> \<forall>t. wellformed_table (db t) (schema t)"
 
-datatype fol_expr = Var nat | Const nat | Neg fol_expr | And fol_expr fol_expr | Or fol_expr fol_expr | Eq fol_expr fol_expr
+fun wellformed_sql_expr :: "sql_expr \<Rightarrow> nat \<Rightarrow> bool" where
+"wellformed_sql_expr (Column i) n = (i < n)" |
+"wellformed_sql_expr (Bin e1 _ e2) n = (wellformed_sql_expr e1 n \<and> wellformed_sql_expr e2 n)" |
+"wellformed_sql_expr _ _ = True"
+
+fun query_output_length :: "query \<Rightarrow> nat" where
+"query_output_length (Table t) = schema t" |
+"query_output_length (Select _ s) = length s"
+
+fun wellformed_query :: "query \<Rightarrow> bool" where
+"wellformed_query (Table _) = True" |
+"wellformed_query (Select q s) = (wellformed_query q \<and> (\<forall>sv\<in>set s. wellformed_sql_expr sv (query_output_length q)))"
+
+datatype fol_expr = Var nat | Const nat | Neg fol_expr | And fol_expr fol_expr |
+  Or fol_expr fol_expr | Eq fol_expr fol_expr | FPlus fol_expr fol_expr | FMinus fol_expr fol_expr
 
 type_synonym fol_env = "nat \<Rightarrow> nat"
 
@@ -38,7 +55,9 @@ fun fol_eval :: "fol_expr \<Rightarrow> fol_env \<Rightarrow> nat" where
 "fol_eval (Neg e) env = bneg (fol_eval e env)" |
 "fol_eval (And e1 e2) env = band (fol_eval e1 env) (fol_eval e2 env)" |
 "fol_eval (Or e1 e2) env = bor (fol_eval e1 env) (fol_eval e2 env)" |
-"fol_eval (Eq e1 e2) env = (if fol_eval e1 env = fol_eval e2 env then 1 else 0)"
+"fol_eval (Eq e1 e2) env = (if fol_eval e1 env = fol_eval e2 env then 1 else 0)" |
+"fol_eval (FPlus e1 e2) env = fol_eval e1 env + fol_eval e2 env" |
+"fol_eval (FMinus e1 e2) env = fol_eval e1 env - fol_eval e2 env"
 
 definition imp :: "fol_expr \<Rightarrow> fol_expr \<Rightarrow> fol_expr" where
 "imp f1 f2 \<equiv> (Or (Neg f1) f2)"
@@ -69,8 +88,29 @@ definition eval_qpsr_table :: "symbolic_column list \<Rightarrow> fol_expr \<Rig
 definition eval_qpsr :: "qpsr \<Rightarrow> qpsr_env \<Rightarrow> (table \<times> table)" where
 "eval_qpsr qpsr env \<equiv> (eval_qpsr_table (cols1 qpsr) (cond qpsr) env, eval_qpsr_table (cols2 qpsr) (cond qpsr) env)"
 
+fun op_op :: "op \<Rightarrow> (nat \<Rightarrow> nat \<Rightarrow> nat)" where
+"op_op Plus = (+)" |
+"op_op Minus = (-)"
+
+fun eval_op :: "op \<Rightarrow> svalue \<Rightarrow> svalue \<Rightarrow> svalue" where
+"eval_op op (SNat n1) (SNat n2) = SNat (op_op op n1 n2)" |
+"eval_op _ _ _ = SNull"
+
+fun select_single :: "sql_expr \<Rightarrow> row \<Rightarrow> svalue" where
+"select_single (Column i) r = r ! i" |
+"select_single (SConst v) _ = SNat v" |
+"select_single Null _ = SNull" |
+"select_single (Bin e1 op e2) r = eval_op op (select_single e1 r) (select_single e2 r)"
+
+definition select_row :: "sql_expr list \<Rightarrow> row \<Rightarrow> row" where
+"select_row s r \<equiv> map (\<lambda>sv. select_single sv r) s"
+
+definition select :: "sql_expr list \<Rightarrow> table \<Rightarrow> table" where
+"select s t \<equiv> image_mset (select_row s) t"
+
 fun eval_query :: "query \<Rightarrow> db \<Rightarrow> table" where
-"eval_query (Table t) db = db t"
+"eval_query (Table t) db = db t" |
+"eval_query (Select q s) db = select s (eval_query q db)"
 
 fun init_tuple :: "nat \<Rightarrow> nat \<Rightarrow> symbolic_column list" where
 "init_tuple _ 0 = []" |
@@ -79,8 +119,29 @@ fun init_tuple :: "nat \<Rightarrow> nat \<Rightarrow> symbolic_column list" whe
 definition veri_table :: "string \<Rightarrow> string \<Rightarrow> qpsr option" where
 "veri_table t1 t2 \<equiv> if t1 = t2 then Some (\<lparr> cols1 = init_tuple 0 (schema t1), cols2 = init_tuple 0 (schema t1), cond = Const 1 \<rparr>) else None"
 
+fun const_op_h :: "op \<Rightarrow> fol_expr \<Rightarrow> fol_expr \<Rightarrow> fol_expr" where
+"const_op_h Plus a b = FPlus a b" |
+"const_op_h Minus a b = FMinus a b"
+
+definition const_op :: "op \<Rightarrow> symbolic_column \<Rightarrow> symbolic_column \<Rightarrow> symbolic_column" where
+"const_op op c1 c2 \<equiv> \<lparr> val = const_op_h op (val c1) (val c2), is_null = Or (is_null c1) (is_null c2) \<rparr>"
+
+fun const_expr :: "symbolic_column list \<Rightarrow> sql_expr \<Rightarrow> symbolic_column" where
+"const_expr cols (Column i) = cols ! i" |
+"const_expr _ (SConst v) = \<lparr> val = Const v, is_null = Const 0 \<rparr>" |
+"const_expr _ Null = \<lparr> val = Const 0, is_null = Const 1 \<rparr>" |
+"const_expr cols (Bin e1 op e2) = const_op op (const_expr cols e1) (const_expr cols e2)"
+
+definition const_expr_list :: "symbolic_column list \<Rightarrow> sql_expr list \<Rightarrow> symbolic_column list" where
+"const_expr_list cols s \<equiv> map (const_expr cols) s"
+
+definition veri_select :: "qpsr \<Rightarrow> sql_expr list \<Rightarrow> sql_expr list \<Rightarrow> qpsr" where
+"veri_select qpsr s1 s2 \<equiv> \<lparr> cols1 = const_expr_list (cols1 qpsr) s1, cols2 = const_expr_list (cols2 qpsr) s2, cond = cond qpsr \<rparr>"
+
 fun veri_card :: "query \<Rightarrow> query \<Rightarrow> qpsr option" where
-"veri_card (Table t1) (Table t2) = veri_table t1 t2"
+"veri_card (Table t1) (Table t2) = veri_table t1 t2" |
+"veri_card (Select q1 s1) (Select q2 s2) = (case veri_card q1 q2 of None \<Rightarrow> None | Some qpsr \<Rightarrow> Some (veri_select qpsr s1 s2))" |
+"veri_card _ _ = None"
 
 definition symbolic_col_eq_expr :: "symbolic_column \<Rightarrow> symbolic_column \<Rightarrow> fol_expr" where
 "symbolic_col_eq_expr c1 c2 \<equiv> Or (And (is_null c1) (is_null c2)) (And (Eq (val c1) (val c2)) (Eq (is_null c1) (is_null c2)))"
@@ -96,12 +157,17 @@ definition qpsr_is_eq :: "qpsr \<Rightarrow> bool" where
 definition spes :: "query \<Rightarrow> query \<Rightarrow> bool" where
 "spes q1 q2 \<equiv> case veri_card q1 q2 of None \<Rightarrow> False | Some qpsr \<Rightarrow> qpsr_is_eq qpsr"
 
-lemma impr:
+lemma imp_elim:
   assumes "fol_eval a env > 0"
   shows "(fol_eval (imp a b) env > 0) = (fol_eval b env > 0)"
   by (metis One_nat_def assms bneg.elims bor.elims fol_eval.simps(3,5) gr0_conv_Suc imp_def)
 
-lemma eval_qpsr_table_row:
+lemma wellformed_query_sub:
+  assumes "wellformed_query (Select q s)"
+  shows "wellformed_query q"
+  by (metis assms wellformed_query.simps(2))
+
+lemma eval_qpsr_table_from_rows:
   assumes "\<forall>r\<in>#t. \<exists>envr. include_qpsr_row condp envr \<and> eval_qpsr_row cols envr = r"
   shows "\<exists>env. eval_qpsr_table cols condp env = t"
 using assms proof (induct t)
@@ -130,7 +196,7 @@ next
   show ?case using head tail by (simp add: eval_qpsr_row_def)
 qed
 
-lemma veri_table_qpsr_h4_gen:
+lemma init_tuple_surj:
   "\<exists>envr. eval_qpsr_row (init_tuple i (length r)) envr = r"
 proof (induct r arbitrary: i)
   case Nil
@@ -160,52 +226,148 @@ next
   then show ?case by auto
 qed
 
-lemma veri_table_qpsr_h4:
-  shows "\<exists>envr. eval_qpsr_row (init_tuple 0 (length r)) envr = r"
-  using veri_table_qpsr_h4_gen by blast
-
-lemma veri_table_qpsr_h3:
+lemma init_tuple_surj_with_cond:
   shows "\<exists>envr. include_qpsr_row (Const 1) envr \<and> eval_qpsr_row (init_tuple 0 (length r)) envr = r"
-  by (simp add: include_qpsr_row_def veri_table_qpsr_h4)
+  by (metis include_qpsr_row_def init_tuple_surj fol_eval.simps(2) less_one)
 
-lemma veri_table_qpsr_h2:
+lemma eval_qpsr_table_surj:
   assumes "wellformed_table x l"
   shows "\<exists>env. eval_qpsr_table (init_tuple 0 l) (Const 1) env = x"
-  by (smt (verit, del_insts) assms eval_qpsr_table_row veri_table_qpsr_h3 wellformed_table_def)
+  by (smt (verit, del_insts) assms eval_qpsr_table_from_rows init_tuple_surj_with_cond wellformed_table_def)
 
-lemma veri_table_qpsr_h:
+lemma eval_qpsr_table_surj_db:
   assumes "wellformed_db db"
   shows "\<exists>env. eval_qpsr_table (init_tuple 0 (schema t)) (Const 1) env = eval_query (Table t) db"
-  by (metis assms veri_table_qpsr_h2 eval_query.simps wellformed_db_def)               
+  by (metis assms eval_qpsr_table_surj wellformed_db_def eval_query.simps(1))
 
-lemma veri_table_qpsr:
+lemma veri_table_correct:
   assumes "wellformed_db db"
   assumes "veri_table t1 t2 = Some qpsr"
   shows "\<exists>env. eval_qpsr qpsr env = (eval_query (Table t1) db, eval_query (Table t2) db)"
-  by (metis assms(1,2) eval_qpsr_def option.distinct(1) option.sel qpsr.ext_inject qpsr.surjective veri_table_def veri_table_qpsr_h)
+  by (metis assms(1,2) eval_qpsr_def option.distinct(1) option.sel qpsr.ext_inject qpsr.surjective veri_table_def eval_qpsr_table_surj_db)
 
-lemma veri_card_qpsr:
-  assumes "wellformed_db db"
-  assumes "veri_card q1 q2 = Some qpsr"
-  shows "\<exists>env. eval_qpsr qpsr env = (eval_query q1 db, eval_query q2 db)"
-using assms proof (induct rule: veri_card.induct)
-  case (1 t1 t2)
+lemma select_image_mset:
+  shows "select s (image_mset f x) = image_mset (\<lambda>r. select_row s (f r)) x"
+  by (metis (no_types, lifting) ext SPES.select_def empty_iff image_mset.compositionality image_mset_single insert_iff set_mset_add_mset_insert set_mset_empty)
+
+lemma eval_qpsr_row_map:
+  shows "eval_qpsr_row (map f x) envr = map (\<lambda>col. eval_symbolic_column (f col) envr) x"
+  using eval_qpsr_row_def by auto
+
+lemma eval_const_op:
+  "eval_symbolic_column (const_op opr c1 c2) envr = eval_op opr (eval_symbolic_column c1 envr) (eval_symbolic_column c2 envr)"
+  unfolding eval_symbolic_column_def const_op_def
+  by (cases "fol_eval (is_null c1) envr"; cases "fol_eval (is_null c2) envr"; cases opr) auto
+
+lemma const_expr_correct:
+  assumes "wellformed_sql_expr sv (length cols)"
+  shows "eval_symbolic_column ((const_expr cols) sv) envr = select_single sv (map (\<lambda>col. eval_symbolic_column col envr) cols)"
+using assms proof (induct sv)
+  case (Column i)
+  have "eval_symbolic_column (cols ! i) envr = (map (\<lambda>col. eval_symbolic_column col envr) cols) ! i"
+    using Column by force
+  then show ?case by simp
+next
+  case (SConst x)
   then show ?case
-    using veri_table_qpsr by auto
+    by (simp add: eval_symbolic_column_def)
+next
+  case Null
+  have "eval_symbolic_column \<lparr> val = Const 0, is_null = Const 1 \<rparr> envr = SNull"
+    by (simp add: eval_symbolic_column_def)
+  then show ?case by simp
+next
+  case (Bin e1 op e2)
+  then show ?case
+    using eval_const_op by force
 qed
 
-lemma qpsr_is_eq_cond_true_h:
-  assumes "qpsr_is_eq qpsr"
-  assumes "include_qpsr_row (cond qpsr) envr"
-  shows "fol_eval (symbolic_cols_eq_expr (cols1 qpsr) (cols2 qpsr)) envr > 0"
-  by (metis assms(2) assms(1) qpsr_is_eq_def include_qpsr_row_def impr)
+lemma const_expr_list_correct_row:
+  assumes "\<forall>sv \<in> set s. wellformed_sql_expr sv (length cols)"
+  shows "eval_qpsr_row (const_expr_list cols s) envr = select_row s (eval_qpsr_row cols envr)"
+  using const_expr_list_def assms const_expr_correct eval_qpsr_row_def select_row_def by simp
 
-lemma qpsr_is_eq_cond_true_h4:
+lemma const_expr_list_correct_table:
+  assumes "\<forall>sv \<in> set s. wellformed_sql_expr sv (length cols)"
+  shows "eval_qpsr_table (const_expr_list cols s) condp env = select s (eval_qpsr_table cols condp env)"
+  by (metis (mono_tags, lifting) assms eval_qpsr_table_def multiset.map_cong select_image_mset const_expr_list_correct_row)
+
+lemma veri_select_correct:
+  assumes "\<forall>sv \<in> set s1. wellformed_sql_expr sv (length (cols1 qpsr))"
+  assumes "\<forall>sv \<in> set s2. wellformed_sql_expr sv (length (cols2 qpsr))"
+  assumes "eval_qpsr qpsr env = (x, y)"
+  shows "eval_qpsr (veri_select qpsr s1 s2) env = (select s1 x, select s2 y)"
+  unfolding eval_qpsr_def
+  using assms eval_qpsr_def veri_select_def const_expr_list_correct_table by auto
+
+lemma veri_select_correct_query:
+  assumes "\<forall>sv \<in> set s1. wellformed_sql_expr sv (length (cols1 qpsr))"
+  assumes "\<forall>sv \<in> set s2. wellformed_sql_expr sv (length (cols2 qpsr))"
+  assumes "eval_qpsr qpsr env = (eval_query q1 db, eval_query q2 db)"
+  shows "eval_qpsr (veri_select qpsr s1 s2) env = (eval_query (Select q1 s1) db, eval_query (Select q2 s2) db)"
+  by (simp add: assms(1,2,3) veri_select_correct)
+
+lemma veri_card_cols_length:
+  assumes "wellformed_query q1"
+  assumes "wellformed_query q2"
+  assumes "veri_card q1 q2 = Some qpsr"
+  shows "length (cols1 qpsr) = query_output_length q1 \<and> length (cols2 qpsr) = query_output_length q2"
+using assms proof (induct rule: veri_card.induct)
+  case (1 t1 t2)
+  have "length (init_tuple 0 (schema t1)) = schema t1"
+    by (metis Ex_list_of_length eval_qpsr_row_def length_map init_tuple_surj)
+  then show ?case
+    by (metis "1.prems"(3) option.distinct(1) option.inject qpsr.ext_inject qpsr.surjective query_output_length.simps(1) veri_card.simps(1) veri_table_def)
+next
+  case (2 q1 s1 q2 s2)
+  obtain qpsr where "veri_card q1 q2 = Some qpsr"
+    using "2.prems"(3) by fastforce
+  have "length (const_expr_list (cols1 qpsr) s1) = query_output_length (Select q1 s1)"
+    using const_expr_list_def by auto
+  have "length (const_expr_list (cols2 qpsr) s2) = query_output_length (Select q2 s2)"
+    by (simp add: const_expr_list_def)
+  then show ?case
+    using "2.prems"(3) \<open>length (const_expr_list (cols1 qpsr) s1) = query_output_length (Select q1 s1)\<close> \<open>veri_card q1 q2 = Some qpsr\<close> veri_select_def by auto
+next
+  case ("3_1" v va vb)
+  then show ?case by simp
+next
+  case ("3_2" vb v va)
+  then show ?case by simp
+qed
+
+lemma veri_card_correct:
+  assumes "wellformed_db db"
+  assumes "wellformed_query q1"
+  assumes "wellformed_query q2"
+  assumes "veri_card q1 q2 = Some qpsr"
+  shows "\<exists>env. eval_qpsr qpsr env = (eval_query q1 db, eval_query q2 db)"
+using assms proof (induct arbitrary: qpsr rule: veri_card.induct)
+  case (1 t1 t2)
+  then show ?case
+    using veri_table_correct by auto
+next
+  case (2 q1 s1 q2 s2)
+  obtain qpsr where "veri_card q1 q2 = Some qpsr"
+    using "2.prems"(4) by fastforce
+  obtain env where "eval_qpsr qpsr env = (eval_query q1 db, eval_query q2 db)"
+    using "2.hyps" "2.prems"(2,3) \<open>veri_card q1 q2 = Some qpsr\<close> assms(1) wellformed_query_sub by blast
+  then show ?case
+    by (smt (verit) "2.prems"(2,3,4) \<open>veri_card q1 q2 = Some qpsr\<close> option.sel option.simps(5) veri_card.simps(2) veri_select_correct_query wellformed_query.simps(2) veri_card_cols_length)
+next
+  case ("3_1" v va vb)
+  then show ?case by simp
+next
+  case ("3_2" vb v va)
+  then show ?case by simp
+qed
+
+lemma symbolic_col_eq_expr_head:
   assumes "fol_eval (symbolic_cols_eq_expr (x#xs) (y#ys)) envr > 0"
   shows "fol_eval (symbolic_col_eq_expr x y) envr > 0"
   by (metis assms band.elims fol_eval.simps(4) gr0_conv_Suc symbolic_cols_eq_expr.simps(2))
 
-lemma qpsr_is_eq_cond_true_h5:
+lemma symbolic_col_eq_expr_correct:
   assumes "fol_eval (symbolic_col_eq_expr x y) envr > 0"
   shows "eval_symbolic_column x envr = eval_symbolic_column y envr"
 proof (cases "fol_eval (And (is_null x) (is_null y)) envr > 0")
@@ -218,12 +380,7 @@ next
     by (metis (no_types, lifting) assms band.elims bor.simps(1) eval_symbolic_column_def fol_eval.simps(4,5,6) gr0_conv_Suc symbolic_col_eq_expr_def)
 qed
 
-lemma qpsr_is_eq_cond_true_h3:
-  assumes "fol_eval (symbolic_cols_eq_expr (x#xs) (y#ys)) envr > 0"
-  shows "eval_symbolic_column x envr = eval_symbolic_column y envr"
-  by (metis assms qpsr_is_eq_cond_true_h5 qpsr_is_eq_cond_true_h4)
-
-lemma qpsr_is_eq_cond_true_h2:
+lemma symbolic_cols_eq_expr_correct:
   assumes "fol_eval (symbolic_cols_eq_expr c1 c2) envr > 0"
   shows "eval_qpsr_row c1 envr = eval_qpsr_row c2 envr"
 using assms proof (induct rule: symbolic_cols_eq_expr.induct)
@@ -232,7 +389,7 @@ using assms proof (induct rule: symbolic_cols_eq_expr.induct)
 next
   case (2 x xs y ys)
   then show ?case
-    using eval_qpsr_row_def qpsr_is_eq_cond_true_h3 by force
+    using eval_qpsr_row_def symbolic_col_eq_expr_correct symbolic_col_eq_expr_head by fastforce
 next
   case ("3_1" v va)
   then show ?case by simp
@@ -241,22 +398,31 @@ next
   then show ?case by simp
 qed
 
-lemma qpsr_is_eq_cond_true:
+lemma qpsr_is_eq_rows_eq:
   assumes "qpsr_is_eq qpsr"
   assumes "include_qpsr_row (cond qpsr) envr"
   shows "eval_qpsr_row (cols1 qpsr) envr = eval_qpsr_row (cols2 qpsr) envr"
-  by (metis assms(2) assms(1) qpsr_is_eq_cond_true_h qpsr_is_eq_cond_true_h2)
+  by (meson SPES.imp_elim assms(1,2) include_qpsr_row_def qpsr_is_eq_def symbolic_cols_eq_expr_correct)
 
 lemma eval_qpsr_eq:
   assumes "eval_qpsr qpsr env = (x, y)"
   assumes "qpsr_is_eq qpsr"
   shows "x = y"
-  by (metis assms(1,2) eval_qpsr_def eval_qpsr_table_def filter_mset_eq_conv fst_conv image_mset_cong qpsr_is_eq_cond_true snd_conv)
+  by (metis assms(1,2) eval_qpsr_def eval_qpsr_table_def filter_mset_eq_conv fst_conv image_mset_cong qpsr_is_eq_rows_eq snd_conv)
 
 theorem spes_sound:
   assumes "wellformed_db db"
+  assumes "wellformed_query q1"
+  assumes "wellformed_query q2"
   assumes "spes q1 q2"
   shows "eval_query q1 db = eval_query q2 db"
-  by (metis assms(1,2) case_optionE eval_qpsr_eq spes_def veri_card_qpsr)
+proof -
+  obtain qpsr where vc: "veri_card q1 q2 = Some qpsr" and eq: "qpsr_is_eq qpsr"
+    using assms(4) unfolding spes_def by (auto split: option.splits)
+  obtain env where "eval_qpsr qpsr env = (eval_query q1 db, eval_query q2 db)"
+    using veri_card_correct[OF assms(1,2,3) vc] by blast
+  then show ?thesis
+    using eval_qpsr_eq eq by auto
+qed
 
 end
